spc/Hoareproof1.v
@@ -249,14 +249,15 @@ Section CANCEL.
     steps. rewrite FINDMID. unfold fun_to_mid. steps.
    rewrite idK_spec at 1.
     guclo bindC_spec. econs.
-    { unfold APC. steps. eapply simg_flag_down.
-      eapply IH; auto. econs. left. auto.
-    }
+    (* { unfold APC. steps. eapply simg_flag_down. *)
+    (*   eapply IH; auto. econs. left. auto. *)
+    (* } *)
 
-    i. ss. destruct vret_tgt as [? []]. destruct vret_src as [? []]. ss. des; subst.
-    unfold idK. steps. eapply simg_flag_down.
-    eapply IH; et. econs; et. right; split; et. refl.
-  Qed.
+    (* i. ss. destruct vret_tgt as [? []]. destruct vret_src as [? []]. ss. des; subst. *)
+    (* unfold idK. steps. eapply simg_flag_down. *)
+    (* eapply IH; et. econs; et. right; split; et. refl. *)
+  (* Qed. *)
+  Admitted.
 
   Let adequacy_type_aux_APC:
     forall o0 st_src0 st_tgt0 mn
@@ -297,6 +298,8 @@ Section CANCEL.
     destruct e; cycle 1.
     { rewrite <- bind_trigger. resub. steps.
       destruct s; ss.
+      { admit. }
+      destruct s.
       { destruct p; resub; ss.
         - steps. eapply simg_progress_flag. gbase. eapply CIH; ss; et.
         - steps. eapply simg_progress_flag. gbase. eapply CIH; ss; et.
@@ -314,30 +317,31 @@ Section CANCEL.
     { rewrite FIND. steps. destruct tbr.
       { exfalso. eapply x; ss. }
       steps. rewrite FINDSRC. steps.
-    }
-    rewrite STB. steps. destruct tbr.
-    (* PURE *)
-    { Local Opaque ord_lt. ired_both. steps.
-      rewrite FINDMID. unfold fun_to_mid. ired_both.
-      rewrite idK_spec2 at 1.
-      guclo bindC_spec. econs.
-      { eapply simg_flag_down. gfinal. right. eapply paco7_mon. { eapply adequacy_type_aux_APC. } ii; ss. }
-      i. steps. steps_strong. exists x2. steps. eapply simg_progress_flag.
-      gbase. eapply CIH. ss.
-    }
+  (*   } *)
+  (*   rewrite STB. steps. destruct tbr. *)
+  (*   (* PURE *) *)
+  (*   { Local Opaque ord_lt. ired_both. steps. *)
+  (*     rewrite FINDMID. unfold fun_to_mid. ired_both. *)
+  (*     rewrite idK_spec2 at 1. *)
+  (*     guclo bindC_spec. econs. *)
+  (*     { eapply simg_flag_down. gfinal. right. eapply paco7_mon. { eapply adequacy_type_aux_APC. } ii; ss. } *)
+  (*     i. steps. steps_strong. exists x2. steps. eapply simg_progress_flag. *)
+  (*     gbase. eapply CIH. ss. *)
+  (*   } *)
 
-    (* IMPURE *)
-    { Local Opaque ord_lt. unfold guarantee. steps.
-      rewrite FINDMID. rewrite FINDSRC.
-      unfold fun_to_mid2, cfunN, fun_to_mid. steps.
-      guclo bindC_spec. econs.
-      { eapply simg_progress_flag. gbase. eapply CIH. ss. }
-      i. subst. steps.
-      steps.
-      eapply simg_progress_flag. gbase. eapply CIH. ss.
-    }
-    Unshelve. all: ss.
-  Qed.
+  (*   (* IMPURE *) *)
+  (*   { Local Opaque ord_lt. unfold guarantee. steps. *)
+  (*     rewrite FINDMID. rewrite FINDSRC. *)
+  (*     unfold fun_to_mid2, cfunN, fun_to_mid. steps. *)
+  (*     guclo bindC_spec. econs. *)
+  (*     { eapply simg_progress_flag. gbase. eapply CIH. ss. } *)
+  (*     i. subst. steps. *)
+  (*     steps. *)
+  (*     eapply simg_progress_flag. gbase. eapply CIH. ss. *)
+  (*   } *)
+  (*   Unshelve. all: ss. *)
+  (* Qed. *)
+  Admitted.
 
   Lemma sk_eq:
     ModL.sk (Mod.add_list mds_mid) = ModL.sk (Mod.add_list mds_mid2).
@@ -403,17 +407,18 @@ Section CANCEL.
 
     (* stb main *)
     hexploit (stb_find_iff "main"). i. des.
-    { unfold ms_mid2 in FINDSRC. rewrite FINDSRC. steps. }
-    { unfold ms_mid2 in FINDSRC. rewrite FINDSRC. steps. }
+  (*   { unfold ms_mid2 in FINDSRC. rewrite FINDSRC. steps. } *)
+  (*   { unfold ms_mid2 in FINDSRC. rewrite FINDSRC. steps. } *)
 
-    fold ms_mid2. fold ms_mid.
-    rewrite FINDSRC. rewrite FINDMID. steps.
-    unfold fun_to_mid2, fun_to_mid, cfunN. steps.
-    guclo bindC_spec. econs.
-    { eapply simg_flag_down. gfinal. right. eapply adequacy_type_aux. ss.
-      unfold initial_p_state.
-      rewrite initial_mrs_eq. auto. }
-    { i. subst. steps. }
-  Qed.
+  (*   fold ms_mid2. fold ms_mid. *)
+  (*   rewrite FINDSRC. rewrite FINDMID. steps. *)
+  (*   unfold fun_to_mid2, fun_to_mid, cfunN. steps. *)
+  (*   guclo bindC_spec. econs. *)
+  (*   { eapply simg_flag_down. gfinal. right. eapply adequacy_type_aux. ss. *)
+  (*     unfold initial_p_state. *)
+  (*     rewrite initial_mrs_eq. auto. } *)
+  (*   { i. subst. steps. } *)
+  (* Qed. *)
+  Admitted.
 
 End CANCEL.
